<?xml version="1.0"?>
<rdf:RDF xmlns="https://endlessforms.info/gdo/gdo.owl/"
     xml:base="https://endlessforms.info/gdo/gdo.owl/"
     xmlns:dc="http://purl.org/dc/elements/1.1/"
     xmlns:obo="http://purl.obolibrary.org/obo/"
     xmlns:owl="http://www.w3.org/2002/07/owl#"
     xmlns:rdf="http://www.w3.org/1999/02/22-rdf-syntax-ns#"
     xmlns:xml="http://www.w3.org/XML/1998/namespace"
     xmlns:xsd="http://www.w3.org/2001/XMLSchema#"
     xmlns:foaf="http://xmlns.com/foaf/0.1/"
     xmlns:rdfs="http://www.w3.org/2000/01/rdf-schema#"
     xmlns:dcterms="http://purl.org/dc/terms/"
     xmlns:is_curated_in_ontology="https://www.ontologyrepository.com/CommonCoreOntologies/is_curated_in_ontology/">
    <owl:Ontology rdf:about="https://endlessforms.info/gdo/gdo.owl">
        <owl:versionIRI rdf:resource="https://endlessforms.info/gdo/releases/gdo-1.0.0.owl"/>
        <dc:description>The Graphic Descriptor Ontology (GDO) is intended for use in describing graphics that represent the form of objects. It uses the language of visual communication, illustration, and technical drawing. The GDO is rooted in the Basic Formal Ontology (BFO) and uses several classes from the Information Entity Ontology of the Common Core Ontologies as a mid-level ontology.</dc:description>
        <dc:title>Graphic Descriptor Ontology (GDO)</dc:title>
        <dcterms:creator>Melissa Clarkson</dcterms:creator>
        <dcterms:license rdf:resource="http://creativecommons.org/licenses/by/4.0/"/>
        <owl:versionInfo>1.0.0</owl:versionInfo>
        <foaf:homepage rdf:resource="https://gdo.endlessforms.info/"/>
    </owl:Ontology>
    


    <!-- 
    ///////////////////////////////////////////////////////////////////////////////////////
    //
    // Annotation properties
    //
    ///////////////////////////////////////////////////////////////////////////////////////
     -->

    


    <!-- http://purl.obolibrary.org/obo/IAO_0000111 -->

    <owl:AnnotationProperty rdf:about="http://purl.obolibrary.org/obo/IAO_0000111">
        <rdfs:isDefinedBy rdf:resource="http://purl.obolibrary.org/obo/iao.owl"/>
        <rdfs:label xml:lang="en">editor preferred term</rdfs:label>
    </owl:AnnotationProperty>
    


    <!-- http://purl.obolibrary.org/obo/IAO_0000112 -->

    <owl:AnnotationProperty rdf:about="http://purl.obolibrary.org/obo/IAO_0000112">
        <rdfs:isDefinedBy rdf:resource="http://purl.obolibrary.org/obo/iao.owl"/>
        <rdfs:label xml:lang="en">example of usage</rdfs:label>
    </owl:AnnotationProperty>
    


    <!-- http://purl.obolibrary.org/obo/IAO_0000115 -->

    <owl:AnnotationProperty rdf:about="http://purl.obolibrary.org/obo/IAO_0000115">
        <rdfs:isDefinedBy rdf:resource="http://purl.obolibrary.org/obo/iao.owl"/>
        <rdfs:label xml:lang="en">definition</rdfs:label>
    </owl:AnnotationProperty>
    


    <!-- http://purl.obolibrary.org/obo/IAO_0000116 -->

    <owl:AnnotationProperty rdf:about="http://purl.obolibrary.org/obo/IAO_0000116">
        <rdfs:isDefinedBy rdf:resource="http://purl.obolibrary.org/obo/iao.owl"/>
        <rdfs:label xml:lang="en">editor note</rdfs:label>
    </owl:AnnotationProperty>
    


    <!-- http://purl.obolibrary.org/obo/IAO_0000117 -->

    <owl:AnnotationProperty rdf:about="http://purl.obolibrary.org/obo/IAO_0000117">
        <rdfs:isDefinedBy rdf:resource="http://purl.obolibrary.org/obo/iao.owl"/>
        <rdfs:label xml:lang="en">term editor</rdfs:label>
    </owl:AnnotationProperty>
    


    <!-- http://purl.obolibrary.org/obo/IAO_0000118 -->

    <owl:AnnotationProperty rdf:about="http://purl.obolibrary.org/obo/IAO_0000118">
        <rdfs:isDefinedBy rdf:resource="http://purl.obolibrary.org/obo/iao.owl"/>
        <rdfs:label xml:lang="en">alternative term</rdfs:label>
    </owl:AnnotationProperty>
    


    <!-- http://purl.obolibrary.org/obo/IAO_0000119 -->

    <owl:AnnotationProperty rdf:about="http://purl.obolibrary.org/obo/IAO_0000119">
        <rdfs:isDefinedBy rdf:resource="http://purl.obolibrary.org/obo/iao.owl"/>
        <rdfs:label xml:lang="en">definition source</rdfs:label>
    </owl:AnnotationProperty>
    


    <!-- http://purl.obolibrary.org/obo/IAO_0000232 -->

    <owl:AnnotationProperty rdf:about="http://purl.obolibrary.org/obo/IAO_0000232">
        <rdfs:isDefinedBy rdf:resource="http://purl.obolibrary.org/obo/iao.owl"/>
        <rdfs:label xml:lang="en">curator note</rdfs:label>
    </owl:AnnotationProperty>
    


    <!-- http://purl.obolibrary.org/obo/IAO_0000412 -->

    <owl:AnnotationProperty rdf:about="http://purl.obolibrary.org/obo/IAO_0000412">
        <rdfs:isDefinedBy rdf:resource="http://purl.obolibrary.org/obo/iao.owl"/>
        <rdfs:label xml:lang="en">imported from</rdfs:label>
    </owl:AnnotationProperty>
    


    <!-- http://purl.obolibrary.org/obo/IAO_0000600 -->

    <owl:AnnotationProperty rdf:about="http://purl.obolibrary.org/obo/IAO_0000600">
        <rdfs:isDefinedBy rdf:resource="http://purl.obolibrary.org/obo/iao.owl"/>
        <rdfs:label xml:lang="en">elucidation</rdfs:label>
    </owl:AnnotationProperty>
    


    <!-- http://purl.org/dc/elements/1.1/contributor -->

    <owl:AnnotationProperty rdf:about="http://purl.org/dc/elements/1.1/contributor"/>
    


    <!-- http://purl.org/dc/elements/1.1/description -->

    <owl:AnnotationProperty rdf:about="http://purl.org/dc/elements/1.1/description"/>
    


    <!-- http://purl.org/dc/elements/1.1/member -->

    <owl:AnnotationProperty rdf:about="http://purl.org/dc/elements/1.1/member"/>
    


    <!-- http://purl.org/dc/elements/1.1/title -->

    <owl:AnnotationProperty rdf:about="http://purl.org/dc/elements/1.1/title"/>
    


    <!-- http://purl.org/dc/terms/creator -->

    <owl:AnnotationProperty rdf:about="http://purl.org/dc/terms/creator"/>
    


    <!-- http://purl.org/dc/terms/license -->

    <owl:AnnotationProperty rdf:about="http://purl.org/dc/terms/license"/>
    


    <!-- http://www.w3.org/2000/01/rdf-schema#isDefinedBy -->

    <owl:AnnotationProperty rdf:about="http://www.w3.org/2000/01/rdf-schema#isDefinedBy"/>
    


    <!-- http://www.w3.org/2000/01/rdf-schema#seeAlso -->

    <owl:AnnotationProperty rdf:about="http://www.w3.org/2000/01/rdf-schema#seeAlso"/>
    


    <!-- http://xmlns.com/foaf/0.1/homepage -->

    <owl:AnnotationProperty rdf:about="http://xmlns.com/foaf/0.1/homepage"/>
    


    <!-- https://www.ontologyrepository.com/CommonCoreOntologies/is_curated_in_ontology/is_curated_in_ontology -->

    <owl:AnnotationProperty rdf:about="https://www.ontologyrepository.com/CommonCoreOntologies/is_curated_in_ontology/is_curated_in_ontology">
        <rdfs:label>is curated in ontology</rdfs:label>
        <is_curated_in_ontology:is_curated_in_ontology>http://www.ontologyrepository.com/CommonCoreOntologies/Mid/ExtendedRelationOntology</is_curated_in_ontology:is_curated_in_ontology>
    </owl:AnnotationProperty>
    


    <!-- 
    ///////////////////////////////////////////////////////////////////////////////////////
    //
    // Object Properties
    //
    ///////////////////////////////////////////////////////////////////////////////////////
     -->

    


    <!-- https://endlessforms.info/gdo/GDO_0000236 -->

    <owl:ObjectProperty rdf:about="https://endlessforms.info/gdo/GDO_0000236">
        <rdfs:domain rdf:resource="https://endlessforms.info/gdo/GDO_0000237"/>
        <obo:IAO_0000115>A relation between a pictoral information bearing entity and a referent, such that the pictoral information bearing entity represents the referent.</obo:IAO_0000115>
        <rdfs:label xml:lang="en">depicts</rdfs:label>
    </owl:ObjectProperty>
    


    <!-- https://endlessforms.info/gdo/GDO_0000239 -->

    <owl:ObjectProperty rdf:about="https://endlessforms.info/gdo/GDO_0000239">
        <rdfs:domain rdf:resource="https://endlessforms.info/gdo/GDO_0000237"/>
        <rdfs:range rdf:resource="https://endlessforms.info/gdo/GDO_0000237"/>
        <obo:IAO_0000115>A relation between two pictoral information bearing entities, such that the same referent is shown in each but from different views.</obo:IAO_0000115>
        <rdfs:label xml:lang="en">displays alternate view of</rdfs:label>
    </owl:ObjectProperty>
    


    <!-- https://endlessforms.info/gdo/GDO_0000240 -->

    <owl:ObjectProperty rdf:about="https://endlessforms.info/gdo/GDO_0000240">
        <rdfs:domain rdf:resource="https://endlessforms.info/gdo/GDO_0000237"/>
        <rdfs:range rdf:resource="https://endlessforms.info/gdo/GDO_0000237"/>
        <obo:IAO_0000115>A relation between two pictorial information bearing entities, such that the feature of interest is shown on the right in one figure and on the left in the other.</obo:IAO_0000115>
        <rdfs:label xml:lang="en">displays opposite laterality to</rdfs:label>
    </owl:ObjectProperty>
    


    <!-- https://endlessforms.info/gdo/GDO_0000241 -->

    <owl:ObjectProperty rdf:about="https://endlessforms.info/gdo/GDO_0000241">
        <owl:inverseOf rdf:resource="https://endlessforms.info/gdo/GDO_0000243"/>
        <rdfs:domain rdf:resource="https://endlessforms.info/gdo/GDO_0000237"/>
        <rdfs:range rdf:resource="http://purl.obolibrary.org/obo/IAO_0000101"/>
        <obo:IAO_0000115>A relation between a graphic and an image, such that the marks of the graphic are interpretations of the boundaries and features of the referent object depicted by the image.</obo:IAO_0000115>
        <rdfs:label xml:lang="en">graphical interpretation of</rdfs:label>
    </owl:ObjectProperty>
    


    <!-- https://endlessforms.info/gdo/GDO_0000242 -->

    <owl:ObjectProperty rdf:about="https://endlessforms.info/gdo/GDO_0000242">
        <rdfs:domain rdf:resource="https://endlessforms.info/gdo/GDO_0000001"/>
        <rdfs:range rdf:resource="https://endlessforms.info/gdo/GDO_0000034"/>
        <obo:IAO_0000115>A relation between a graphic and a graphic style, such that the graphic is drawn using this graphic style.</obo:IAO_0000115>
        <rdfs:label xml:lang="en">has graphic style</rdfs:label>
    </owl:ObjectProperty>
    


    <!-- https://endlessforms.info/gdo/GDO_0000243 -->

    <owl:ObjectProperty rdf:about="https://endlessforms.info/gdo/GDO_0000243">
        <rdfs:domain rdf:resource="http://purl.obolibrary.org/obo/IAO_0000101"/>
        <rdfs:range rdf:resource="https://endlessforms.info/gdo/GDO_0000001"/>
        <obo:IAO_0000115>A relation between an image and a graphic, such that variations of color and luminosity within the image representing boundaries and features of the referent object have been depicted as marks within the graphic.</obo:IAO_0000115>
        <rdfs:label xml:lang="en">has graphical interpretation</rdfs:label>
    </owl:ObjectProperty>
    


    <!-- https://endlessforms.info/gdo/GDO_0000244 -->

    <owl:ObjectProperty rdf:about="https://endlessforms.info/gdo/GDO_0000244">
        <rdfs:domain rdf:resource="https://endlessforms.info/gdo/GDO_0000001"/>
        <rdfs:range rdf:resource="https://endlessforms.info/gdo/GDO_0000037"/>
        <obo:IAO_0000115>A relation between a graphic and a projection type, such that the graphic was created using this projection type.</obo:IAO_0000115>
        <rdfs:label xml:lang="en">has projection type</rdfs:label>
    </owl:ObjectProperty>
    


    <!-- https://endlessforms.info/gdo/GDO_0000245 -->

    <owl:ObjectProperty rdf:about="https://endlessforms.info/gdo/GDO_0000245">
        <rdfs:domain rdf:resource="https://endlessforms.info/gdo/GDO_0000237"/>
        <rdfs:range rdf:resource="https://endlessforms.info/gdo/GDO_0000016"/>
        <obo:IAO_0000115>A relation between a pictoral information bearing entity and a view, such that the pictoral information bearing entity depicts the referent from this view.</obo:IAO_0000115>
        <rdfs:label xml:lang="en">has view</rdfs:label>
    </owl:ObjectProperty>
    


    <!-- 
    ///////////////////////////////////////////////////////////////////////////////////////
    //
    // Data properties
    //
    ///////////////////////////////////////////////////////////////////////////////////////
     -->

    


    <!-- https://endlessforms.info/gdo/GDO_0000246 -->

    <owl:DatatypeProperty rdf:about="https://endlessforms.info/gdo/GDO_0000246">
        <rdfs:domain rdf:resource="https://endlessforms.info/gdo/GDO_0000237"/>
        <rdfs:range>
            <rdfs:Datatype>
                <owl:oneOf>
                    <rdf:Description>
                        <rdf:type rdf:resource="http://www.w3.org/1999/02/22-rdf-syntax-ns#List"/>
                        <rdf:first>bilateral</rdf:first>
                        <rdf:rest>
                            <rdf:Description>
                                <rdf:type rdf:resource="http://www.w3.org/1999/02/22-rdf-syntax-ns#List"/>
                                <rdf:first>left</rdf:first>
                                <rdf:rest>
                                    <rdf:Description>
                                        <rdf:type rdf:resource="http://www.w3.org/1999/02/22-rdf-syntax-ns#List"/>
                                        <rdf:first>right</rdf:first>
                                        <rdf:rest rdf:resource="http://www.w3.org/1999/02/22-rdf-syntax-ns#nil"/>
                                    </rdf:Description>
                                </rdf:rest>
                            </rdf:Description>
                        </rdf:rest>
                    </rdf:Description>
                </owl:oneOf>
            </rdfs:Datatype>
        </rdfs:range>
        <obo:IAO_0000115>The laterality of the structure or feature of interest.</obo:IAO_0000115>
        <rdfs:label xml:lang="en">depicts feature laterality</rdfs:label>
    </owl:DatatypeProperty>
    


    <!-- https://endlessforms.info/gdo/GDO_0000247 -->

    <owl:DatatypeProperty rdf:about="https://endlessforms.info/gdo/GDO_0000247">
        <rdfs:domain rdf:resource="https://endlessforms.info/gdo/GDO_0000237"/>
        <rdfs:range rdf:resource="http://www.w3.org/2001/XMLSchema#float"/>
        <obo:IAO_0000115>The angle of rotation of the referent around an axis vertical to the viewer.</obo:IAO_0000115>
        <rdfs:label xml:lang="en">depicts rotation</rdfs:label>
    </owl:DatatypeProperty>
    


    <!-- https://endlessforms.info/gdo/GDO_0000248 -->

    <owl:DatatypeProperty rdf:about="https://endlessforms.info/gdo/GDO_0000248">
        <rdfs:domain rdf:resource="https://endlessforms.info/gdo/GDO_0000237"/>
        <rdfs:range rdf:resource="http://www.w3.org/2001/XMLSchema#float"/>
        <obo:IAO_0000115>The angle of rotation of the referent around an axis that extends to the left and right of the viewer and is horizontal.</obo:IAO_0000115>
        <rdfs:label xml:lang="en">depicts slant</rdfs:label>
    </owl:DatatypeProperty>
    


    <!-- https://endlessforms.info/gdo/GDO_0000249 -->

    <owl:DatatypeProperty rdf:about="https://endlessforms.info/gdo/GDO_0000249">
        <rdfs:domain rdf:resource="https://endlessforms.info/gdo/GDO_0000237"/>
        <rdfs:range rdf:resource="http://www.w3.org/2001/XMLSchema#float"/>
        <obo:IAO_0000115>The angle of rotation of the referent around the axis that is the viewer&apos;s line of sight.</obo:IAO_0000115>
        <rdfs:label xml:lang="en">depicts tilt</rdfs:label>
    </owl:DatatypeProperty>
    


    <!-- 
    ///////////////////////////////////////////////////////////////////////////////////////
    //
    // Classes
    //
    ///////////////////////////////////////////////////////////////////////////////////////
     -->

    


    <!-- http://purl.obolibrary.org/obo/BFO_0000001 -->

    <owl:Class rdf:about="http://purl.obolibrary.org/obo/BFO_0000001">
        <rdfs:subClassOf rdf:resource="http://www.w3.org/2002/07/owl#Thing"/>
        <obo:IAO_0000600 xml:lang="en">An entity is anything that exists or has existed or will exist. (axiom label in BFO2 Reference: [001-001])</obo:IAO_0000600>
        <rdfs:isDefinedBy rdf:resource="http://purl.obolibrary.org/obo/bfo.owl"/>
        <rdfs:label xml:lang="en">entity</rdfs:label>
        <is_curated_in_ontology:is_curated_in_ontology>http://purl.obolibrary.org/obo/bfo.owl</is_curated_in_ontology:is_curated_in_ontology>
    </owl:Class>
    


    <!-- http://purl.obolibrary.org/obo/BFO_0000002 -->

    <owl:Class rdf:about="http://purl.obolibrary.org/obo/BFO_0000002">
        <rdfs:subClassOf rdf:resource="http://purl.obolibrary.org/obo/BFO_0000001"/>
        <obo:IAO_0000600 xml:lang="en">A continuant is an entity that persists, endures, or continues to exist through time while maintaining its identity. (axiom label in BFO2 Reference: [008-002])</obo:IAO_0000600>
        <rdfs:isDefinedBy rdf:resource="http://purl.obolibrary.org/obo/bfo.owl"/>
        <rdfs:label xml:lang="en">continuant</rdfs:label>
        <is_curated_in_ontology:is_curated_in_ontology>http://purl.obolibrary.org/obo/bfo.owl</is_curated_in_ontology:is_curated_in_ontology>
    </owl:Class>
    


    <!-- http://purl.obolibrary.org/obo/BFO_0000004 -->

    <owl:Class rdf:about="http://purl.obolibrary.org/obo/BFO_0000004">
        <rdfs:subClassOf rdf:resource="http://purl.obolibrary.org/obo/BFO_0000002"/>
        <owl:disjointWith rdf:resource="http://purl.obolibrary.org/obo/BFO_0000020"/>
        <owl:disjointWith rdf:resource="http://purl.obolibrary.org/obo/BFO_0000031"/>
        <obo:IAO_0000115 xml:lang="en">b is an independent continuant = Def. b is a continuant which is such that there is no c and no t such that b s-depends_on c at t. (axiom label in BFO2 Reference: [017-002])</obo:IAO_0000115>
        <rdfs:isDefinedBy rdf:resource="http://purl.obolibrary.org/obo/bfo.owl"/>
        <rdfs:label xml:lang="en">independent continuant</rdfs:label>
        <is_curated_in_ontology:is_curated_in_ontology>http://purl.obolibrary.org/obo/bfo.owl</is_curated_in_ontology:is_curated_in_ontology>
    </owl:Class>
    


    <!-- http://purl.obolibrary.org/obo/BFO_0000017 -->

    <owl:Class rdf:about="http://purl.obolibrary.org/obo/BFO_0000017">
        <rdfs:subClassOf rdf:resource="http://purl.obolibrary.org/obo/BFO_0000020"/>
        <owl:disjointWith rdf:resource="http://purl.obolibrary.org/obo/BFO_0000019"/>
        <obo:IAO_0000600 xml:lang="en">To say that b is a realizable entity is to say that b is a specifically dependent continuant that inheres in some independent continuant which is not a spatial region and is of a type instances of which are realized in processes of a correlated type. (axiom label in BFO2 Reference: [058-002])</obo:IAO_0000600>
        <rdfs:isDefinedBy rdf:resource="http://purl.obolibrary.org/obo/bfo.owl"/>
        <rdfs:label xml:lang="en">realizable entity</rdfs:label>
        <is_curated_in_ontology:is_curated_in_ontology>http://purl.obolibrary.org/obo/bfo.owl</is_curated_in_ontology:is_curated_in_ontology>
    </owl:Class>
    


    <!-- http://purl.obolibrary.org/obo/BFO_0000019 -->

    <owl:Class rdf:about="http://purl.obolibrary.org/obo/BFO_0000019">
        <rdfs:subClassOf rdf:resource="http://purl.obolibrary.org/obo/BFO_0000020"/>
        <obo:IAO_0000600 xml:lang="en">a quality is a specifically dependent continuant that, in contrast to roles and dispositions, does not require any further process in order to be realized. (axiom label in BFO2 Reference: [055-001])</obo:IAO_0000600>
        <rdfs:isDefinedBy rdf:resource="http://purl.obolibrary.org/obo/bfo.owl"/>
        <rdfs:label xml:lang="en">quality</rdfs:label>
        <is_curated_in_ontology:is_curated_in_ontology>http://purl.obolibrary.org/obo/bfo.owl</is_curated_in_ontology:is_curated_in_ontology>
    </owl:Class>
    


    <!-- http://purl.obolibrary.org/obo/BFO_0000020 -->

    <owl:Class rdf:about="http://purl.obolibrary.org/obo/BFO_0000020">
        <rdfs:subClassOf rdf:resource="http://purl.obolibrary.org/obo/BFO_0000002"/>
        <owl:disjointWith rdf:resource="http://purl.obolibrary.org/obo/BFO_0000031"/>
        <obo:IAO_0000115 xml:lang="en">b is a specifically dependent continuant = Def. b is a continuant &amp; there is some independent continuant c which is not a spatial region and which is such that b s-depends_on c at every time t during the course of b’s existence. (axiom label in BFO2 Reference: [050-003])</obo:IAO_0000115>
        <rdfs:isDefinedBy rdf:resource="http://purl.obolibrary.org/obo/bfo.owl"/>
        <rdfs:label xml:lang="en">specifically dependent continuant</rdfs:label>
        <is_curated_in_ontology:is_curated_in_ontology>http://purl.obolibrary.org/obo/bfo.owl</is_curated_in_ontology:is_curated_in_ontology>
    </owl:Class>
    


    <!-- http://purl.obolibrary.org/obo/BFO_0000023 -->

    <owl:Class rdf:about="http://purl.obolibrary.org/obo/BFO_0000023">
        <rdfs:subClassOf rdf:resource="http://purl.obolibrary.org/obo/BFO_0000017"/>
        <obo:IAO_0000600 xml:lang="en">b is a role means: b is a realizable entity &amp; b exists because there is some single bearer that is in some special physical, social, or institutional set of circumstances in which this bearer does not have to be&amp; b is not such that, if it ceases to exist, then the physical make-up of the bearer is thereby changed. (axiom label in BFO2 Reference: [061-001])</obo:IAO_0000600>
        <rdfs:isDefinedBy rdf:resource="http://purl.obolibrary.org/obo/bfo.owl"/>
        <rdfs:label xml:lang="en">role</rdfs:label>
        <is_curated_in_ontology:is_curated_in_ontology>http://purl.obolibrary.org/obo/bfo.owl</is_curated_in_ontology:is_curated_in_ontology>
    </owl:Class>
    


    <!-- http://purl.obolibrary.org/obo/BFO_0000030 -->

    <owl:Class rdf:about="http://purl.obolibrary.org/obo/BFO_0000030">
        <rdfs:subClassOf rdf:resource="http://purl.obolibrary.org/obo/BFO_0000040"/>
        <rdfs:isDefinedBy rdf:resource="http://purl.obolibrary.org/obo/bfo.owl"/>
        <rdfs:label xml:lang="en">object</rdfs:label>
        <is_curated_in_ontology:is_curated_in_ontology>http://purl.obolibrary.org/obo/bfo.owl</is_curated_in_ontology:is_curated_in_ontology>
    </owl:Class>
    


    <!-- http://purl.obolibrary.org/obo/BFO_0000031 -->

    <owl:Class rdf:about="http://purl.obolibrary.org/obo/BFO_0000031">
        <rdfs:subClassOf rdf:resource="http://purl.obolibrary.org/obo/BFO_0000002"/>
        <obo:IAO_0000115 xml:lang="en">b is a generically dependent continuant = Def. b is a continuant that g-depends_on one or more other entities. (axiom label in BFO2 Reference: [074-001])</obo:IAO_0000115>
        <rdfs:isDefinedBy rdf:resource="http://purl.obolibrary.org/obo/bfo.owl"/>
        <rdfs:label xml:lang="en">generically dependent continuant</rdfs:label>
        <is_curated_in_ontology:is_curated_in_ontology>http://purl.obolibrary.org/obo/bfo.owl</is_curated_in_ontology:is_curated_in_ontology>
    </owl:Class>
    


    <!-- http://purl.obolibrary.org/obo/BFO_0000040 -->

    <owl:Class rdf:about="http://purl.obolibrary.org/obo/BFO_0000040">
        <rdfs:subClassOf rdf:resource="http://purl.obolibrary.org/obo/BFO_0000004"/>
        <obo:IAO_0000600 xml:lang="en">A material entity is an independent continuant that has some portion of matter as proper or improper continuant part. (axiom label in BFO2 Reference: [019-002])</obo:IAO_0000600>
        <rdfs:isDefinedBy rdf:resource="http://purl.obolibrary.org/obo/bfo.owl"/>
        <rdfs:label xml:lang="en">material entity</rdfs:label>
        <is_curated_in_ontology:is_curated_in_ontology>http://purl.obolibrary.org/obo/bfo.owl</is_curated_in_ontology:is_curated_in_ontology>
    </owl:Class>
    


    <!-- http://purl.obolibrary.org/obo/IAO_0000101 -->

    <owl:Class rdf:about="http://purl.obolibrary.org/obo/IAO_0000101">
        <rdfs:subClassOf rdf:resource="https://endlessforms.info/gdo/GDO_0000237"/>
        <obo:IAO_0000115>An image is an affine projection to a two dimensional surface, of measurements of some quality of an entity or entities repeated at regular intervals across a spatial range, where the measurements are represented as color and luminosity on the projected on surface.</obo:IAO_0000115>
        <obo:IAO_0000116>This class includes photographs, radiographs, and micrographs.</obo:IAO_0000116>
        <rdfs:label xml:lang="en">image</rdfs:label>
        <is_curated_in_ontology:is_curated_in_ontology>https://github.com/information-artifact-ontology/IAO/</is_curated_in_ontology:is_curated_in_ontology>
    </owl:Class>
    


    <!-- http://www.ontologyrepository.com/CommonCoreOntologies/DirectiveInformationContentEntity -->

    <owl:Class rdf:about="http://www.ontologyrepository.com/CommonCoreOntologies/DirectiveInformationContentEntity">
        <rdfs:subClassOf rdf:resource="http://www.ontologyrepository.com/CommonCoreOntologies/InformationContentEntity"/>
        <obo:IAO_0000115>An Information Content Entity that consists of a set of propositions or images (as in the case of a blueprint) that prescribe some Entity.</obo:IAO_0000115>
        <rdfs:label xml:lang="en">directive information content entity</rdfs:label>
        <is_curated_in_ontology:is_curated_in_ontology>http://www.ontologyrepository.com/CommonCoreOntologies/Mid/InformationEntityOntology</is_curated_in_ontology:is_curated_in_ontology>
    </owl:Class>
    


    <!-- http://www.ontologyrepository.com/CommonCoreOntologies/InformationBearingEntity -->

    <owl:Class rdf:about="http://www.ontologyrepository.com/CommonCoreOntologies/InformationBearingEntity">
        <rdfs:subClassOf rdf:resource="http://purl.obolibrary.org/obo/BFO_0000030"/>
        <obo:IAO_0000115>An object upon which an information content entity generically depends.</obo:IAO_0000115>
        <rdfs:label xml:lang="en">information bearing entity</rdfs:label>
        <is_curated_in_ontology:is_curated_in_ontology>http://www.ontologyrepository.com/CommonCoreOntologies/Mid/InformationEntityOntology</is_curated_in_ontology:is_curated_in_ontology>
    </owl:Class>
    


    <!-- http://www.ontologyrepository.com/CommonCoreOntologies/InformationContentEntity -->

    <owl:Class rdf:about="http://www.ontologyrepository.com/CommonCoreOntologies/InformationContentEntity">
        <rdfs:subClassOf rdf:resource="http://purl.obolibrary.org/obo/BFO_0000031"/>
        <obo:IAO_0000115>A Generically Dependent Continuant that generically depends on some Information Bearing Entity and stands in relation of aboutness to some Entity.</obo:IAO_0000115>
        <rdfs:label xml:lang="en">information content entity</rdfs:label>
        <is_curated_in_ontology:is_curated_in_ontology>http://www.ontologyrepository.com/CommonCoreOntologies/Mid/InformationEntityOntology</is_curated_in_ontology:is_curated_in_ontology>
    </owl:Class>
    


    <!-- http://www.ontologyrepository.com/CommonCoreOntologies/RepresentationalInformationContentEntity -->

    <owl:Class rdf:about="http://www.ontologyrepository.com/CommonCoreOntologies/RepresentationalInformationContentEntity">
        <rdfs:subClassOf rdf:resource="http://www.ontologyrepository.com/CommonCoreOntologies/InformationContentEntity"/>
        <obo:IAO_0000115>An Information Content Entity that represents some Entity.</obo:IAO_0000115>
        <rdfs:label xml:lang="en">representational information content entity</rdfs:label>
        <is_curated_in_ontology:is_curated_in_ontology>http://www.ontologyrepository.com/CommonCoreOntologies/Mid/InformationEntityOntology</is_curated_in_ontology:is_curated_in_ontology>
    </owl:Class>
    


    <!-- https://endlessforms.info/gdo/GDO_0000001 -->

    <owl:Class rdf:about="https://endlessforms.info/gdo/GDO_0000001">
        <rdfs:subClassOf rdf:resource="https://endlessforms.info/gdo/GDO_0000237"/>
        <obo:IAO_0000115>A pictoral information bearing entity that is a pictorial model of a referent composed of graphical marks that are designed to be interpreted as corresponding to the form (spatial properties) of the referent. The referent may be an object referent or conceptual referent.</obo:IAO_0000115>
        <obo:IAO_0000232>This definition includes both visual graphics and tactile graphics.</obo:IAO_0000232>
        <rdfs:label xml:lang="en">graphic</rdfs:label>
    </owl:Class>
    


    <!-- https://endlessforms.info/gdo/GDO_0000002 -->

    <owl:Class rdf:about="https://endlessforms.info/gdo/GDO_0000002">
        <rdfs:subClassOf rdf:resource="https://endlessforms.info/gdo/GDO_0000001"/>
        <owl:disjointWith rdf:resource="https://endlessforms.info/gdo/GDO_0000003"/>
        <obo:IAO_0000115>A graphic consisting of marks positioned using a two-dimensional (planar) coordinate system.</obo:IAO_0000115>
        <rdfs:label xml:lang="en">2D graphic</rdfs:label>
    </owl:Class>
    


    <!-- https://endlessforms.info/gdo/GDO_0000003 -->

    <owl:Class rdf:about="https://endlessforms.info/gdo/GDO_0000003">
        <rdfs:subClassOf rdf:resource="https://endlessforms.info/gdo/GDO_0000001"/>
        <obo:IAO_0000115>A graphic consisting of marks positioned using a three-dimensional (volumetric) coordinate system but projected onto a 2D plane by a computer system for display.</obo:IAO_0000115>
        <rdfs:label xml:lang="en">3D graphic</rdfs:label>
    </owl:Class>
    


    <!-- https://endlessforms.info/gdo/GDO_0000004 -->

    <owl:Class rdf:about="https://endlessforms.info/gdo/GDO_0000004">
        <rdfs:subClassOf rdf:resource="https://endlessforms.info/gdo/GDO_0000001"/>
        <owl:disjointWith rdf:resource="https://endlessforms.info/gdo/GDO_0000005"/>
        <obo:IAO_0000115>A graphic designed with raised surfaces to be perceived using touch.</obo:IAO_0000115>
        <rdfs:label xml:lang="en">tactile graphic</rdfs:label>
    </owl:Class>
    


    <!-- https://endlessforms.info/gdo/GDO_0000005 -->

    <owl:Class rdf:about="https://endlessforms.info/gdo/GDO_0000005">
        <rdfs:subClassOf rdf:resource="https://endlessforms.info/gdo/GDO_0000001"/>
        <obo:IAO_0000115>A graphic designed to be perceived using sight.</obo:IAO_0000115>
        <rdfs:label xml:lang="en">visual graphic</rdfs:label>
    </owl:Class>
    


    <!-- https://endlessforms.info/gdo/GDO_0000006 -->

    <owl:Class rdf:about="https://endlessforms.info/gdo/GDO_0000006">
        <rdfs:subClassOf rdf:resource="https://endlessforms.info/gdo/GDO_0000237"/>
        <obo:IAO_0000115>A pictoral information bearing entity that is a fundamental unit of representation within a graphic. A graphical mark can be perceptually segmented from the other elements of the graphic based on the mark’s color or luminosity (for a visual graphic) or raised surface (for a tactile graphic). A composition of graphical marks constitutes a graphic.</obo:IAO_0000115>
        <rdfs:label xml:lang="en">graphical mark</rdfs:label>
    </owl:Class>
    


    <!-- https://endlessforms.info/gdo/GDO_0000007 -->

    <owl:Class rdf:about="https://endlessforms.info/gdo/GDO_0000007">
        <rdfs:subClassOf rdf:resource="https://endlessforms.info/gdo/GDO_0000006"/>
        <obo:IAO_0000115>A graphical mark that rendered within a two- or three-dimensional coordinate system that evokes recognition of a two-dimensional surface or three-dimensional volume by the human perceptual system.</obo:IAO_0000115>
        <rdfs:label xml:lang="en">region mark</rdfs:label>
    </owl:Class>
    


    <!-- https://endlessforms.info/gdo/GDO_0000008 -->

    <owl:Class rdf:about="https://endlessforms.info/gdo/GDO_0000008">
        <rdfs:subClassOf rdf:resource="https://endlessforms.info/gdo/GDO_0000006"/>
        <obo:IAO_0000115>A graphical mark rendered within a two- or three-dimensional coordinate system that evokes recognition of a one-dimensional line by the human perceptual system.</obo:IAO_0000115>
        <rdfs:label xml:lang="en">line mark</rdfs:label>
    </owl:Class>
    


    <!-- https://endlessforms.info/gdo/GDO_0000009 -->

    <owl:Class rdf:about="https://endlessforms.info/gdo/GDO_0000009">
        <rdfs:subClassOf rdf:resource="https://endlessforms.info/gdo/GDO_0000006"/>
        <obo:IAO_0000115>A graphical mark rendered within a two- or three-dimensional coordinate system that evokes recognition of a position (rather than an extent) by the human perceptual system.</obo:IAO_0000115>
        <rdfs:label xml:lang="en">point mark</rdfs:label>
    </owl:Class>
    


    <!-- https://endlessforms.info/gdo/GDO_0000010 -->

    <owl:Class rdf:about="https://endlessforms.info/gdo/GDO_0000010">
        <rdfs:subClassOf rdf:resource="https://endlessforms.info/gdo/GDO_0000237"/>
        <obo:IAO_0000115>A pictoral information bearing entity that is a contiguous area within a graphic.</obo:IAO_0000115>
        <rdfs:label xml:lang="en">region of graphic</rdfs:label>
    </owl:Class>
    


    <!-- https://endlessforms.info/gdo/GDO_0000011 -->

    <owl:Class rdf:about="https://endlessforms.info/gdo/GDO_0000011">
        <rdfs:subClassOf rdf:resource="https://endlessforms.info/gdo/GDO_0000010"/>
        <obo:IAO_0000115>A region of a graphic containing the graphical marks that represent the subject matter of a graphic.</obo:IAO_0000115>
        <rdfs:label xml:lang="en">foreground of graphic</rdfs:label>
    </owl:Class>
    


    <!-- https://endlessforms.info/gdo/GDO_0000012 -->

    <owl:Class rdf:about="https://endlessforms.info/gdo/GDO_0000012">
        <rdfs:subClassOf rdf:resource="https://endlessforms.info/gdo/GDO_0000010"/>
        <obo:IAO_0000115>A region of a graphic that is not the foreground. The background may contain no graphical marks or may contain marks that do not represent the main subject of the communication.</obo:IAO_0000115>
        <rdfs:label xml:lang="en">background of graphic</rdfs:label>
    </owl:Class>
    


    <!-- https://endlessforms.info/gdo/GDO_0000013 -->

    <owl:Class rdf:about="https://endlessforms.info/gdo/GDO_0000013">
        <rdfs:subClassOf rdf:resource="https://endlessforms.info/gdo/GDO_0000010"/>
        <obo:IAO_0000115>A region of a graphic that is deemed to be particularly important for the communication purpose of the graphic.</obo:IAO_0000115>
        <rdfs:label xml:lang="en">region of interest of graphic</rdfs:label>
    </owl:Class>
    


    <!-- https://endlessforms.info/gdo/GDO_0000014 -->

    <owl:Class rdf:about="https://endlessforms.info/gdo/GDO_0000014">
        <rdfs:subClassOf rdf:resource="http://purl.obolibrary.org/obo/BFO_0000019"/>
        <obo:IAO_0000115>A quality of a pictorial information content entity.</obo:IAO_0000115>
        <rdfs:label xml:lang="en">pictorial quality</rdfs:label>
    </owl:Class>
    


    <!-- https://endlessforms.info/gdo/GDO_0000015 -->

    <owl:Class rdf:about="https://endlessforms.info/gdo/GDO_0000015">
        <rdfs:subClassOf rdf:resource="http://www.ontologyrepository.com/CommonCoreOntologies/RepresentationalInformationContentEntity"/>
        <obo:IAO_0000115>A representational information content entity for which the information is primarily about the form (spatial properties) and appearance of one or more referents.</obo:IAO_0000115>
        <rdfs:label xml:lang="en">pictorial information content entity</rdfs:label>
    </owl:Class>
    


    <!-- https://endlessforms.info/gdo/GDO_0000016 -->

    <owl:Class rdf:about="https://endlessforms.info/gdo/GDO_0000016">
        <rdfs:subClassOf rdf:resource="https://endlessforms.info/gdo/GDO_0000014"/>
        <obo:IAO_0000115>A pictorial quality that describes the positional relation between the referent and the line of sight of the viewer within the scene that is depicted.</obo:IAO_0000115>
        <rdfs:label xml:lang="en">view</rdfs:label>
    </owl:Class>
    


    <!-- https://endlessforms.info/gdo/GDO_0000018 -->

    <owl:Class rdf:about="https://endlessforms.info/gdo/GDO_0000018">
        <rdfs:subClassOf rdf:resource="https://endlessforms.info/gdo/GDO_0000016"/>
        <obo:IAO_0000115>A view that depicts one of the six faces of a referent drawn using an orthographic projection.</obo:IAO_0000115>
        <rdfs:label xml:lang="en">orthographic view</rdfs:label>
    </owl:Class>
    


    <!-- https://endlessforms.info/gdo/GDO_0000026 -->

    <owl:Class rdf:about="https://endlessforms.info/gdo/GDO_0000026">
        <rdfs:subClassOf rdf:resource="https://endlessforms.info/gdo/GDO_0000014"/>
        <obo:IAO_0000115>A pictorial quality that describes the techniqe used to make parts of a referent visible that would not otherwise be visible to a viewer.</obo:IAO_0000115>
        <rdfs:label xml:lang="en">style of representation of parts</rdfs:label>
    </owl:Class>
    


    <!-- https://endlessforms.info/gdo/GDO_0000032 -->

    <owl:Class rdf:about="https://endlessforms.info/gdo/GDO_0000032">
        <rdfs:subClassOf rdf:resource="http://purl.obolibrary.org/obo/BFO_0000030"/>
        <obo:IAO_0000115>The object that a representation represents. A object referent may be a particular object in the world or a class of objects.</obo:IAO_0000115>
        <rdfs:comment>A referent is either an object referent or a conceptual referent.</rdfs:comment>
        <rdfs:label xml:lang="en">object referent</rdfs:label>
    </owl:Class>
    


    <!-- https://endlessforms.info/gdo/GDO_0000033 -->

    <owl:Class rdf:about="https://endlessforms.info/gdo/GDO_0000033">
        <rdfs:subClassOf rdf:resource="http://purl.obolibrary.org/obo/BFO_0000031"/>
        <obo:IAO_0000115>An entity conceptualized in the mind that a representation represents.</obo:IAO_0000115>
        <rdfs:comment>A referent is either an object referent or a conceptual referent.</rdfs:comment>
        <rdfs:label xml:lang="en">conceptual referent</rdfs:label>
    </owl:Class>
    


    <!-- https://endlessforms.info/gdo/GDO_0000034 -->

    <owl:Class rdf:about="https://endlessforms.info/gdo/GDO_0000034">
        <rdfs:subClassOf rdf:resource="https://endlessforms.info/gdo/GDO_0000014"/>
        <obo:IAO_0000115>A pictoral quality that describes the manner in which a graphic depicts the referent.</obo:IAO_0000115>
        <rdfs:label xml:lang="en">graphic style</rdfs:label>
    </owl:Class>
    


    <!-- https://endlessforms.info/gdo/GDO_0000037 -->

    <owl:Class rdf:about="https://endlessforms.info/gdo/GDO_0000037">
        <rdfs:subClassOf rdf:resource="https://endlessforms.info/gdo/GDO_0000014"/>
        <obo:IAO_0000115>A pictoral quality that describes the technique employed for representing a three-dimensional referent as a two-dimensional graphic.</obo:IAO_0000115>
        <rdfs:label xml:lang="en">projection type</rdfs:label>
    </owl:Class>
    


    <!-- https://endlessforms.info/gdo/GDO_0000038 -->

    <owl:Class rdf:about="https://endlessforms.info/gdo/GDO_0000038">
        <rdfs:subClassOf rdf:resource="https://endlessforms.info/gdo/GDO_0000037"/>
        <obo:IAO_0000115>A projection type for which the lines of sight (imaginary lines extending from the referent to viewer of the referent) are parallel to each other, as if the viewer is at an infinite distance. Parallel projections are most commonly used in engineering applications because they preserve the geometry of the object depicted.</obo:IAO_0000115>
        <rdfs:label xml:lang="en">parallel projection</rdfs:label>
    </owl:Class>
    


    <!-- https://endlessforms.info/gdo/GDO_0000041 -->

    <owl:Class rdf:about="https://endlessforms.info/gdo/GDO_0000041">
        <rdfs:subClassOf rdf:resource="https://endlessforms.info/gdo/GDO_0000037"/>
        <obo:IAO_0000115>A projection type for which the lines of sight (imaginary straight lines extending from the referent to viewer of the referent) converge at the viewer’s eye (known as the center of projection). Perspective projections are most commonly used in artistic and illustration applications because they mimic the optical effect of receding lines.</obo:IAO_0000115>
        <rdfs:label xml:lang="en">perspective projection</rdfs:label>
    </owl:Class>
    


    <!-- https://endlessforms.info/gdo/GDO_0000045 -->

    <owl:Class rdf:about="https://endlessforms.info/gdo/GDO_0000045">
        <rdfs:subClassOf rdf:resource="http://purl.obolibrary.org/obo/BFO_0000019"/>
        <obo:IAO_0000115>A quality that describes a graphical mark.</obo:IAO_0000115>
        <rdfs:label xml:lang="en">graphical mark quality</rdfs:label>
    </owl:Class>
    


    <!-- https://endlessforms.info/gdo/GDO_0000046 -->

    <owl:Class rdf:about="https://endlessforms.info/gdo/GDO_0000046">
        <rdfs:subClassOf rdf:resource="https://endlessforms.info/gdo/GDO_0000045"/>
        <obo:IAO_0000115>A graphical mark quality that describes the lightness or darkness of a mark.</obo:IAO_0000115>
        <rdfs:label xml:lang="en">value of graphical mark</rdfs:label>
    </owl:Class>
    


    <!-- https://endlessforms.info/gdo/GDO_0000047 -->

    <owl:Class rdf:about="https://endlessforms.info/gdo/GDO_0000047">
        <rdfs:subClassOf rdf:resource="https://endlessforms.info/gdo/GDO_0000046"/>
        <obo:IAO_0000115>A value of a graphical mark with the quality of having no wavelengths of light reflected or transmitted such that it is perceived as maximum darkness.</obo:IAO_0000115>
        <rdfs:label xml:lang="en">black value</rdfs:label>
    </owl:Class>
    


    <!-- https://endlessforms.info/gdo/GDO_0000048 -->

    <owl:Class rdf:about="https://endlessforms.info/gdo/GDO_0000048">
        <rdfs:subClassOf rdf:resource="https://endlessforms.info/gdo/GDO_0000046"/>
        <obo:IAO_0000115>A value of a graphical mark with the quality of having all wavelengths of light reflected or transmitted equally (therefore being achromatic, or without hue) such that it is perceived as darker than a mark with a dark value but lighter than a mark with a black value.</obo:IAO_0000115>
        <rdfs:comment>A nine-step value scale was devised by Denman Ross in the early 1900s with seven ordered tones between white and black. The seven values are high light, light, low light, middle value, high dark, dark, and low dark.

https://archive.org/details/theoryofpuredesi00rossuoft/page/134</rdfs:comment>
        <rdfs:label xml:lang="en">low dark value of Denman Ross value scale</rdfs:label>
    </owl:Class>
    


    <!-- https://endlessforms.info/gdo/GDO_0000049 -->

    <owl:Class rdf:about="https://endlessforms.info/gdo/GDO_0000049">
        <rdfs:subClassOf rdf:resource="https://endlessforms.info/gdo/GDO_0000046"/>
        <obo:IAO_0000115>A value of a graphical mark with the quality of having all wavelengths of light reflected or transmitted equally (therefore being achromatic, or without hue) such that it is perceived as darker than a mark with a high dark value but lighter than a mark with a low dark value.</obo:IAO_0000115>
        <rdfs:comment>A nine-step value scale was devised by Denman Ross in the early 1900s with seven ordered tones between white and black. The seven values are high light, light, low light, middle value, high dark, dark, and low dark.

https://archive.org/details/theoryofpuredesi00rossuoft/page/134</rdfs:comment>
        <rdfs:label xml:lang="en">dark value of Denman Ross scale</rdfs:label>
    </owl:Class>
    


    <!-- https://endlessforms.info/gdo/GDO_0000050 -->

    <owl:Class rdf:about="https://endlessforms.info/gdo/GDO_0000050">
        <rdfs:subClassOf rdf:resource="https://endlessforms.info/gdo/GDO_0000046"/>
        <obo:IAO_0000115>A value of a graphical mark with the quality of having all wavelengths of light reflected or transmitted equally (therefore being achromatic, or without hue) such that it is perceived as darker than a mark with a middle value but lighter than a mark with a dark value.</obo:IAO_0000115>
        <rdfs:comment>A nine-step value scale was devised by Denman Ross in the early 1900s with seven ordered tones between white and black. The seven values are high light, light, low light, middle value, high dark, dark, and low dark.

https://archive.org/details/theoryofpuredesi00rossuoft/page/134</rdfs:comment>
        <rdfs:label xml:lang="en">high dark value of Denman Ross value scale</rdfs:label>
    </owl:Class>
    


    <!-- https://endlessforms.info/gdo/GDO_0000051 -->

    <owl:Class rdf:about="https://endlessforms.info/gdo/GDO_0000051">
        <rdfs:subClassOf rdf:resource="https://endlessforms.info/gdo/GDO_0000046"/>
        <obo:IAO_0000115>A value of a graphical mark with the quality of having all wavelengths of light reflected or transmitted equally (therefore being achromatic, or without hue) such that it is perceived as darker than a mark with a low light value but lighter than a mark with a high dark value.</obo:IAO_0000115>
        <rdfs:comment>A nine-step value scale was devised by Denman Ross in the early 1900s with seven ordered tones between white and black. The seven values are high light, light, low light, middle value, high dark, dark, and low dark.

https://archive.org/details/theoryofpuredesi00rossuoft/page/134</rdfs:comment>
        <rdfs:label xml:lang="en">middle value of Denman Ross value scale</rdfs:label>
    </owl:Class>
    


    <!-- https://endlessforms.info/gdo/GDO_0000052 -->

    <owl:Class rdf:about="https://endlessforms.info/gdo/GDO_0000052">
        <rdfs:subClassOf rdf:resource="https://endlessforms.info/gdo/GDO_0000046"/>
        <obo:IAO_0000115>A value of a graphical mark with the quality of having all wavelengths of light reflected or transmitted equally (therefore being achromatic, or without hue) such that it is perceived as darker than a mark with a light value but lighter than a mark with a middle value.</obo:IAO_0000115>
        <rdfs:comment>A nine-step value scale was devised by Denman Ross in the early 1900s with seven ordered tones between white and black. The seven values are high light, light, low light, middle value, high dark, dark, and low dark.

https://archive.org/details/theoryofpuredesi00rossuoft/page/134</rdfs:comment>
        <rdfs:label xml:lang="en">low light value of Denman Ross value scale</rdfs:label>
    </owl:Class>
    


    <!-- https://endlessforms.info/gdo/GDO_0000053 -->

    <owl:Class rdf:about="https://endlessforms.info/gdo/GDO_0000053">
        <rdfs:subClassOf rdf:resource="https://endlessforms.info/gdo/GDO_0000046"/>
        <obo:IAO_0000115>A value of a graphical mark with the quality of having all wavelengths of light reflected or transmitted equally (therefore being achromatic, or without hue) such that it is perceived as darker than a mark with a high light value but lighter than a mark with a low light value.</obo:IAO_0000115>
        <rdfs:comment>A nine-step value scale was devised by Denman Ross in the early 1900s with seven ordered tones between white and black. The seven values are high light, light, low light, middle value, high dark, dark, and low dark.

https://archive.org/details/theoryofpuredesi00rossuoft/page/134</rdfs:comment>
        <rdfs:label xml:lang="en">light value of Denman Ross value scale</rdfs:label>
    </owl:Class>
    


    <!-- https://endlessforms.info/gdo/GDO_0000054 -->

    <owl:Class rdf:about="https://endlessforms.info/gdo/GDO_0000054">
        <rdfs:subClassOf rdf:resource="https://endlessforms.info/gdo/GDO_0000046"/>
        <obo:IAO_0000115>A value of a graphical mark with the quality of having all wavelengths of light reflected or transmitted equally (therefore being achromatic, or without hue) such that it is perceived as darker than a mark with a white value but lighter than a mark with a light value.</obo:IAO_0000115>
        <rdfs:comment>A nine-step value scale was devised by Denman Ross in the early 1900s with seven ordered tones between white and black. The seven values are high light, light, low light, middle value, high dark, dark, and low dark.

https://archive.org/details/theoryofpuredesi00rossuoft/page/134</rdfs:comment>
        <rdfs:label xml:lang="en">high light value of Denman Ross value scale</rdfs:label>
    </owl:Class>
    


    <!-- https://endlessforms.info/gdo/GDO_0000055 -->

    <owl:Class rdf:about="https://endlessforms.info/gdo/GDO_0000055">
        <rdfs:subClassOf rdf:resource="https://endlessforms.info/gdo/GDO_0000046"/>
        <obo:IAO_0000115>A value of a graphical mark with the quality of having all wavelengths of light reflected or transmitted equally (therefore being achromatic, or without hue) such that it is perceived as maximum brightness.</obo:IAO_0000115>
        <rdfs:label xml:lang="en">white value</rdfs:label>
    </owl:Class>
    


    <!-- https://endlessforms.info/gdo/GDO_0000056 -->

    <owl:Class rdf:about="https://endlessforms.info/gdo/GDO_0000056">
        <rdfs:subClassOf rdf:resource="https://endlessforms.info/gdo/GDO_0000045"/>
        <obo:IAO_0000115>A graphical mark quality that describes the level of visual hierarchy of a graphical mark in a graphic.</obo:IAO_0000115>
        <rdfs:label xml:lang="en">level of visual hierarchy of graphical mark</rdfs:label>
    </owl:Class>
    


    <!-- https://endlessforms.info/gdo/GDO_0000057 -->

    <owl:Class rdf:about="https://endlessforms.info/gdo/GDO_0000057">
        <rdfs:subClassOf rdf:resource="https://endlessforms.info/gdo/GDO_0000056"/>
        <obo:IAO_0000115>A level of visual hierarchy of a graphical mark that is less dominant than the tertiary level.</obo:IAO_0000115>
        <rdfs:label xml:lang="en">quaternary level of visual hierarchy</rdfs:label>
    </owl:Class>
    


    <!-- https://endlessforms.info/gdo/GDO_0000058 -->

    <owl:Class rdf:about="https://endlessforms.info/gdo/GDO_0000058">
        <rdfs:subClassOf rdf:resource="https://endlessforms.info/gdo/GDO_0000056"/>
        <obo:IAO_0000115>A level of visual hierarchy of a graphical mark that is less dominant than the secondary level.</obo:IAO_0000115>
        <rdfs:label xml:lang="en">tertiary level of visual hierarchy</rdfs:label>
    </owl:Class>
    


    <!-- https://endlessforms.info/gdo/GDO_0000059 -->

    <owl:Class rdf:about="https://endlessforms.info/gdo/GDO_0000059">
        <rdfs:subClassOf rdf:resource="https://endlessforms.info/gdo/GDO_0000056"/>
        <obo:IAO_0000115>A level of visual hierarchy of a graphical mark that is less dominant than the primary level.</obo:IAO_0000115>
        <rdfs:label xml:lang="en">secondary level of visual hierarchy</rdfs:label>
    </owl:Class>
    


    <!-- https://endlessforms.info/gdo/GDO_0000060 -->

    <owl:Class rdf:about="https://endlessforms.info/gdo/GDO_0000060">
        <rdfs:subClassOf rdf:resource="https://endlessforms.info/gdo/GDO_0000056"/>
        <obo:IAO_0000115>A level of visual hierarchy of a graphical mark that is most dominant in the graphic.</obo:IAO_0000115>
        <rdfs:label xml:lang="en">primary level of visual hierarchy</rdfs:label>
    </owl:Class>
    


    <!-- https://endlessforms.info/gdo/GDO_0000061 -->

    <owl:Class rdf:about="https://endlessforms.info/gdo/GDO_0000061">
        <rdfs:subClassOf rdf:resource="http://purl.obolibrary.org/obo/BFO_0000023"/>
        <obo:IAO_0000115>A role that is a representational purpose of a point mark.</obo:IAO_0000115>
        <rdfs:label xml:lang="en">point mark role</rdfs:label>
    </owl:Class>
    


    <!-- https://endlessforms.info/gdo/GDO_0000062 -->

    <owl:Class rdf:about="https://endlessforms.info/gdo/GDO_0000062">
        <rdfs:subClassOf rdf:resource="https://endlessforms.info/gdo/GDO_0000061"/>
        <obo:IAO_0000115>A point mark role that indicates location.</obo:IAO_0000115>
        <rdfs:label xml:lang="en">location point</rdfs:label>
    </owl:Class>
    


    <!-- https://endlessforms.info/gdo/GDO_0000063 -->

    <owl:Class rdf:about="https://endlessforms.info/gdo/GDO_0000063">
        <rdfs:subClassOf rdf:resource="https://endlessforms.info/gdo/GDO_0000061"/>
        <obo:IAO_0000115>A point mark role that creates tone or texture within a graphic when grouped with other stipples.</obo:IAO_0000115>
        <rdfs:label xml:lang="en">stipple</rdfs:label>
    </owl:Class>
    


    <!-- https://endlessforms.info/gdo/GDO_0000064 -->

    <owl:Class rdf:about="https://endlessforms.info/gdo/GDO_0000064">
        <rdfs:subClassOf rdf:resource="http://purl.obolibrary.org/obo/BFO_0000023"/>
        <obo:IAO_0000115>A role that is a representational purpose of a line mark.</obo:IAO_0000115>
        <rdfs:label xml:lang="en">line mark role</rdfs:label>
    </owl:Class>
    


    <!-- https://endlessforms.info/gdo/GDO_0000065 -->

    <owl:Class rdf:about="https://endlessforms.info/gdo/GDO_0000065">
        <rdfs:subClassOf rdf:resource="https://endlessforms.info/gdo/GDO_0000064"/>
        <obo:IAO_0000115>A line mark role that assists in establishing the three-dimensional nature of the space in which a referent resides.</obo:IAO_0000115>
        <rdfs:label xml:lang="en">construction line</rdfs:label>
    </owl:Class>
    


    <!-- https://endlessforms.info/gdo/GDO_0000066 -->

    <owl:Class rdf:about="https://endlessforms.info/gdo/GDO_0000066">
        <rdfs:subClassOf rdf:resource="https://endlessforms.info/gdo/GDO_0000065"/>
        <obo:IAO_0000115>A construction line that assists in depicting a local plane, arc, or volume that relates to the form, orientation, or coordinate system of the referent. Bounding boxes and depictions of planes are composed of scaffold lines.</obo:IAO_0000115>
        <rdfs:label xml:lang="en">scaffold line</rdfs:label>
    </owl:Class>
    


    <!-- https://endlessforms.info/gdo/GDO_0000067 -->

    <owl:Class rdf:about="https://endlessforms.info/gdo/GDO_0000067">
        <rdfs:subClassOf rdf:resource="https://endlessforms.info/gdo/GDO_0000065"/>
        <obo:IAO_0000115>A construction line that helps to establish the three-dimensional location of an edge, corner, or other feature of the referent for a given type of projection.</obo:IAO_0000115>
        <rdfs:label xml:lang="en">projection line</rdfs:label>
    </owl:Class>
    


    <!-- https://endlessforms.info/gdo/GDO_0000068 -->

    <owl:Class rdf:about="https://endlessforms.info/gdo/GDO_0000068">
        <rdfs:subClassOf rdf:resource="https://endlessforms.info/gdo/GDO_0000065"/>
        <obo:IAO_0000115>A construction line that depicts an axis of the local coordinate system of the referent.</obo:IAO_0000115>
        <rdfs:label xml:lang="en">axis line</rdfs:label>
    </owl:Class>
    


    <!-- https://endlessforms.info/gdo/GDO_0000069 -->

    <owl:Class rdf:about="https://endlessforms.info/gdo/GDO_0000069">
        <rdfs:subClassOf rdf:resource="https://endlessforms.info/gdo/GDO_0000064"/>
        <obo:IAO_0000115>A line mark role that depicts the form or part of the form of a referent.</obo:IAO_0000115>
        <rdfs:label xml:lang="en">form line</rdfs:label>
    </owl:Class>
    


    <!-- https://endlessforms.info/gdo/GDO_0000070 -->

    <owl:Class rdf:about="https://endlessforms.info/gdo/GDO_0000070">
        <rdfs:subClassOf rdf:resource="https://endlessforms.info/gdo/GDO_0000069"/>
        <obo:IAO_0000115>A form line that represents locally maximal changes in surface orientation of the referent.</obo:IAO_0000115>
        <rdfs:label xml:lang="en">crease line</rdfs:label>
    </owl:Class>
    


    <!-- https://endlessforms.info/gdo/GDO_0000071 -->

    <owl:Class rdf:about="https://endlessforms.info/gdo/GDO_0000071">
        <rdfs:subClassOf rdf:resource="https://endlessforms.info/gdo/GDO_0000070"/>
        <obo:IAO_0000115>A crease line that represents the line joining the lowest points of a valley on the surface of the referent.</obo:IAO_0000115>
        <rdfs:label xml:lang="en">valley line</rdfs:label>
    </owl:Class>
    


    <!-- https://endlessforms.info/gdo/GDO_0000072 -->

    <owl:Class rdf:about="https://endlessforms.info/gdo/GDO_0000072">
        <rdfs:subClassOf rdf:resource="https://endlessforms.info/gdo/GDO_0000070"/>
        <obo:IAO_0000115>A crease line that represents the line joining the highest points of a ridge on the surface of the referent.</obo:IAO_0000115>
        <rdfs:label xml:lang="en">ridge line</rdfs:label>
    </owl:Class>
    


    <!-- https://endlessforms.info/gdo/GDO_0000073 -->

    <owl:Class rdf:about="https://endlessforms.info/gdo/GDO_0000073">
        <rdfs:subClassOf rdf:resource="https://endlessforms.info/gdo/GDO_0000069"/>
        <obo:IAO_0000115>A form line that depicts the topology of a surface of a referent by representing the intersection of the surface with an invisible plane.</obo:IAO_0000115>
        <rdfs:label xml:lang="en">cross-contour line</rdfs:label>
    </owl:Class>
    


    <!-- https://endlessforms.info/gdo/GDO_0000074 -->

    <owl:Class rdf:about="https://endlessforms.info/gdo/GDO_0000074">
        <rdfs:subClassOf rdf:resource="https://endlessforms.info/gdo/GDO_0000069"/>
        <obo:IAO_0000115>A form line that depicts an edge resulting from cutting away part of the referent.</obo:IAO_0000115>
        <obo:IAO_0000118>cut margin</obo:IAO_0000118>
        <rdfs:label xml:lang="en">cutaway line</rdfs:label>
    </owl:Class>
    


    <!-- https://endlessforms.info/gdo/GDO_0000075 -->

    <owl:Class rdf:about="https://endlessforms.info/gdo/GDO_0000075">
        <rdfs:subClassOf rdf:resource="https://endlessforms.info/gdo/GDO_0000069"/>
        <obo:IAO_0000115>A form line that delimits regions of surfaces visible to the viewer of the referent from regions of surfaces hidden from the viewer.</obo:IAO_0000115>
        <rdfs:label xml:lang="en">occluding contour line</rdfs:label>
    </owl:Class>
    


    <!-- https://endlessforms.info/gdo/GDO_0000076 -->

    <owl:Class rdf:about="https://endlessforms.info/gdo/GDO_0000076">
        <rdfs:subClassOf rdf:resource="https://endlessforms.info/gdo/GDO_0000069"/>
        <obo:IAO_0000115>A form line that depicts the margin of a depression, cavity, or passage.</obo:IAO_0000115>
        <rdfs:label xml:lang="en">rim line</rdfs:label>
    </owl:Class>
    


    <!-- https://endlessforms.info/gdo/GDO_0000077 -->

    <owl:Class rdf:about="https://endlessforms.info/gdo/GDO_0000077">
        <rdfs:subClassOf rdf:resource="https://endlessforms.info/gdo/GDO_0000064"/>
        <obo:IAO_0000115>A line mark role that, when grouped with other hatch lines, creates a region in a graphic perceived as being a different value or having texture. Groups of hatch lines may depict a surface of the referent or its shadow. When representing a surface, the position of a hatch line depicts the intersection of the surface of the referent object with an in invisible plane. Hatch lines are typically positioned approximately parallel to one another, although they may cross one another to create to intensify the value.</obo:IAO_0000115>
        <rdfs:label xml:lang="en">hatch line</rdfs:label>
    </owl:Class>
    


    <!-- https://endlessforms.info/gdo/GDO_0000078 -->

    <owl:Class rdf:about="https://endlessforms.info/gdo/GDO_0000078">
        <rdfs:subClassOf rdf:resource="https://endlessforms.info/gdo/GDO_0000064"/>
        <obo:IAO_0000115>A line mark role that provides information relevant to understanding the meaning and context of the graphic, rather than information about the form or features of the referent.</obo:IAO_0000115>
        <rdfs:label xml:lang="en">line for annotation of meaning</rdfs:label>
    </owl:Class>
    


    <!-- https://endlessforms.info/gdo/GDO_0000079 -->

    <owl:Class rdf:about="https://endlessforms.info/gdo/GDO_0000079">
        <rdfs:subClassOf rdf:resource="https://endlessforms.info/gdo/GDO_0000078"/>
        <obo:IAO_0000115>A line for annotation of meaning that indicates a relationship between parts of a graphic or between different graphics in a scene.</obo:IAO_0000115>
        <rdfs:label xml:lang="en">connector line</rdfs:label>
    </owl:Class>
    


    <!-- https://endlessforms.info/gdo/GDO_0000080 -->

    <owl:Class rdf:about="https://endlessforms.info/gdo/GDO_0000080">
        <rdfs:subClassOf rdf:resource="https://endlessforms.info/gdo/GDO_0000078"/>
        <obo:IAO_0000115>A line for annotation of meaning that represents a measurable extent (such as length or height) of an object. A dimension line is often drawn using arrowheads and may be bounded with extent lines.</obo:IAO_0000115>
        <rdfs:label xml:lang="en">dimension line</rdfs:label>
    </owl:Class>
    


    <!-- https://endlessforms.info/gdo/GDO_0000081 -->

    <owl:Class rdf:about="https://endlessforms.info/gdo/GDO_0000081">
        <rdfs:subClassOf rdf:resource="https://endlessforms.info/gdo/GDO_0000078"/>
        <obo:IAO_0000115>A line for annotation of meaning that establishes one endpoint of a measurable extent and is oriented perpendicular to the line segment representing the extent (which may or may not be drawn). The distance between a pair of extent lines represents the length of the extent. Extent lines may be used to annotate a dimension of a graphic or a scale line.</obo:IAO_0000115>
        <rdfs:label xml:lang="en">extent line</rdfs:label>
    </owl:Class>
    


    <!-- https://endlessforms.info/gdo/GDO_0000082 -->

    <owl:Class rdf:about="https://endlessforms.info/gdo/GDO_0000082">
        <rdfs:subClassOf rdf:resource="https://endlessforms.info/gdo/GDO_0000078"/>
        <obo:IAO_0000115>A line for annotation of meaning that establishes a relation between part of a graphic and explanatory information in the form of a label, symbol, or another graphic.</obo:IAO_0000115>
        <rdfs:label xml:lang="en">leader line</rdfs:label>
    </owl:Class>
    


    <!-- https://endlessforms.info/gdo/GDO_0000083 -->

    <owl:Class rdf:about="https://endlessforms.info/gdo/GDO_0000083">
        <rdfs:subClassOf rdf:resource="https://endlessforms.info/gdo/GDO_0000098"/>
        <obo:IAO_0000115>A line indicating a path that signifies a path of movement of a referent or a part of a referent. This directed line typically is represented with an arrow.</obo:IAO_0000115>
        <rdfs:label xml:lang="en">line indicating a path of movement</rdfs:label>
    </owl:Class>
    


    <!-- https://endlessforms.info/gdo/GDO_0000084 -->

    <owl:Class rdf:about="https://endlessforms.info/gdo/GDO_0000084">
        <rdfs:subClassOf rdf:resource="https://endlessforms.info/gdo/GDO_0000078"/>
        <obo:IAO_0000115>A line for annotation of meaning that establishes a unit of measurement (or multiples of a unit of measurement) representing the real-world dimensions of the referent. A scale line informs the viewer how much larger or smaller the graphic is drawn relative to the size of the referent in the real world.</obo:IAO_0000115>
        <rdfs:label xml:lang="en">scale line</rdfs:label>
    </owl:Class>
    


    <!-- https://endlessforms.info/gdo/GDO_0000085 -->

    <owl:Class rdf:about="https://endlessforms.info/gdo/GDO_0000085">
        <rdfs:subClassOf rdf:resource="https://endlessforms.info/gdo/GDO_0000064"/>
        <obo:IAO_0000115>A line mark role that provides information about the spatial characteristics of the referent beyond the information depicted using form lines.</obo:IAO_0000115>
        <rdfs:label xml:lang="en">line for annotation of form</rdfs:label>
    </owl:Class>
    


    <!-- https://endlessforms.info/gdo/GDO_0000086 -->

    <owl:Class rdf:about="https://endlessforms.info/gdo/GDO_0000086">
        <rdfs:subClassOf rdf:resource="https://endlessforms.info/gdo/GDO_0000085"/>
        <obo:IAO_0000115>A line for annotation of form that indicates that the form of the referent is not depicted beyond the line.</obo:IAO_0000115>
        <rdfs:label xml:lang="en">discontinuation line</rdfs:label>
    </owl:Class>
    


    <!-- https://endlessforms.info/gdo/GDO_0000087 -->

    <owl:Class rdf:about="https://endlessforms.info/gdo/GDO_0000087">
        <rdfs:subClassOf rdf:resource="https://endlessforms.info/gdo/GDO_0000085"/>
        <obo:IAO_0000115>A line for annotation of form that represents an edge of the referent if the referent was to undergo a change in form, size, or location.</obo:IAO_0000115>
        <rdfs:label xml:lang="en">phantom line</rdfs:label>
    </owl:Class>
    


    <!-- https://endlessforms.info/gdo/GDO_0000088 -->

    <owl:Class rdf:about="https://endlessforms.info/gdo/GDO_0000088">
        <rdfs:subClassOf rdf:resource="https://endlessforms.info/gdo/GDO_0000085"/>
        <obo:IAO_0000115>A line for annotation of form that demarcates sections or regions of a referent.</obo:IAO_0000115>
        <rdfs:label xml:lang="en">sectional line</rdfs:label>
    </owl:Class>
    


    <!-- https://endlessforms.info/gdo/GDO_0000089 -->

    <owl:Class rdf:about="https://endlessforms.info/gdo/GDO_0000089">
        <rdfs:subClassOf rdf:resource="https://endlessforms.info/gdo/GDO_0000064"/>
        <obo:IAO_0000115>A line mark role that represents a discontinuity that appears as a line (or similar to a line) on the referent.</obo:IAO_0000115>
        <rdfs:label xml:lang="en">line of discontinuity</rdfs:label>
    </owl:Class>
    


    <!-- https://endlessforms.info/gdo/GDO_0000090 -->

    <owl:Class rdf:about="https://endlessforms.info/gdo/GDO_0000090">
        <rdfs:subClassOf rdf:resource="https://endlessforms.info/gdo/GDO_0000089"/>
        <obo:IAO_0000115>A line of discontinuity that represents a discontinuity in the color of the referent.</obo:IAO_0000115>
        <rdfs:label xml:lang="en">line of discontinuity of color</rdfs:label>
    </owl:Class>
    


    <!-- https://endlessforms.info/gdo/GDO_0000091 -->

    <owl:Class rdf:about="https://endlessforms.info/gdo/GDO_0000091">
        <rdfs:subClassOf rdf:resource="https://endlessforms.info/gdo/GDO_0000089"/>
        <obo:IAO_0000115>A line of discontinuity that represents a discontinuity of the luminosity of the light on the referent object or background.</obo:IAO_0000115>
        <rdfs:label xml:lang="en">line of discontinuity of light</rdfs:label>
    </owl:Class>
    


    <!-- https://endlessforms.info/gdo/GDO_0000092 -->

    <owl:Class rdf:about="https://endlessforms.info/gdo/GDO_0000092">
        <rdfs:subClassOf rdf:resource="https://endlessforms.info/gdo/GDO_0000089"/>
        <obo:IAO_0000115>A line of discontinuity that represents a discontinuity in a surface of the referent, such as a crack or where surfaces of two objects or parts abut.</obo:IAO_0000115>
        <rdfs:label xml:lang="en">line of discontinuity of plane of surface</rdfs:label>
    </owl:Class>
    


    <!-- https://endlessforms.info/gdo/GDO_0000093 -->

    <owl:Class rdf:about="https://endlessforms.info/gdo/GDO_0000093">
        <rdfs:subClassOf rdf:resource="https://endlessforms.info/gdo/GDO_0000089"/>
        <obo:IAO_0000115>A line of discontinuity that represents a discontinuity in the texture of referent.</obo:IAO_0000115>
        <rdfs:label xml:lang="en">line of discontinuity of texture</rdfs:label>
    </owl:Class>
    


    <!-- https://endlessforms.info/gdo/GDO_0000094 -->

    <owl:Class rdf:about="https://endlessforms.info/gdo/GDO_0000094">
        <rdfs:subClassOf rdf:resource="https://endlessforms.info/gdo/GDO_0000064"/>
        <obo:IAO_0000115>A line mark role that indicates the directionality of bundles, channels, or grooves in a material.</obo:IAO_0000115>
        <rdfs:label xml:lang="en">line of striation</rdfs:label>
    </owl:Class>
    


    <!-- https://endlessforms.info/gdo/GDO_0000095 -->

    <owl:Class rdf:about="https://endlessforms.info/gdo/GDO_0000095">
        <rdfs:subClassOf rdf:resource="https://endlessforms.info/gdo/GDO_0000064"/>
        <obo:IAO_0000115>A line mark role that indicates that the form or feature represented by the line is hidden from the viewer based on the view of the referent that is depicted.</obo:IAO_0000115>
        <rdfs:label xml:lang="en">occluded line</rdfs:label>
    </owl:Class>
    


    <!-- https://endlessforms.info/gdo/GDO_0000096 -->

    <owl:Class rdf:about="https://endlessforms.info/gdo/GDO_0000096">
        <rdfs:subClassOf rdf:resource="http://purl.obolibrary.org/obo/BFO_0000023"/>
        <obo:IAO_0000115>A role that is the representational purpose of a region mark.</obo:IAO_0000115>
        <rdfs:label xml:lang="en">region mark role</rdfs:label>
    </owl:Class>
    


    <!-- https://endlessforms.info/gdo/GDO_0000097 -->

    <owl:Class rdf:about="https://endlessforms.info/gdo/GDO_0000097">
        <rdfs:subClassOf rdf:resource="https://endlessforms.info/gdo/GDO_0000069"/>
        <obo:IAO_0000115>A form line that depicts the form of referent that is not the main subject, and is positioned to provide context or a comparison of form. Examples of use include (a) showing the position of the surface of the object when the subject matter is an internal part, and (b) creating an overlay that compares the size or form of the subject referent to some other referent.</obo:IAO_0000115>
        <rdfs:label xml:lang="en">reference form line</rdfs:label>
    </owl:Class>
    


    <!-- https://endlessforms.info/gdo/GDO_0000098 -->

    <owl:Class rdf:about="https://endlessforms.info/gdo/GDO_0000098">
        <rdfs:subClassOf rdf:resource="https://endlessforms.info/gdo/GDO_0000064"/>
        <obo:IAO_0000115>A line mark role that signifyies a path using a directed line.</obo:IAO_0000115>
        <rdfs:label xml:lang="en">line indicating a path</rdfs:label>
    </owl:Class>
    


    <!-- https://endlessforms.info/gdo/GDO_0000099 -->

    <owl:Class rdf:about="https://endlessforms.info/gdo/GDO_0000099">
        <rdfs:subClassOf rdf:resource="https://endlessforms.info/gdo/GDO_0000098"/>
        <obo:IAO_0000115>A line indicating a path that signifies a path through the space surrounded a referent or through a referent. This directed line is typically is represented with an arrow.</obo:IAO_0000115>
        <rdfs:label xml:lang="en">line indicating a path through space</rdfs:label>
    </owl:Class>
    


    <!-- https://endlessforms.info/gdo/GDO_0000100 -->

    <owl:Class rdf:about="https://endlessforms.info/gdo/GDO_0000100">
        <rdfs:subClassOf rdf:resource="https://endlessforms.info/gdo/GDO_0000078"/>
        <obo:IAO_0000115>A line for annotation of meaning that forms an arrow or part of an arrow that points to a part of a graphic or indicates a direction.</obo:IAO_0000115>
        <rdfs:label xml:lang="en">line of pointer arrow</rdfs:label>
    </owl:Class>
    


    <!-- https://endlessforms.info/gdo/GDO_0000101 -->

    <owl:Class rdf:about="https://endlessforms.info/gdo/GDO_0000101">
        <rdfs:subClassOf rdf:resource="https://endlessforms.info/gdo/GDO_0000078"/>
        <obo:IAO_0000115>A line for annotation of meaning that demarcates a unit of length on a scale. Often used in combination with a scale line, where each scale increment line is perpendicular to the scale line.</obo:IAO_0000115>
        <rdfs:label xml:lang="en">scale increment line</rdfs:label>
    </owl:Class>
    


    <!-- https://endlessforms.info/gdo/GDO_0000179 -->

    <owl:Class rdf:about="https://endlessforms.info/gdo/GDO_0000179">
        <rdfs:subClassOf rdf:resource="https://endlessforms.info/gdo/GDO_0000096"/>
        <obo:IAO_0000115>A region mark role for which the mark designates an area deemed to be particularly important for the communication purpose of the graphic.</obo:IAO_0000115>
        <rdfs:label xml:lang="en">region representing a region of interest</rdfs:label>
    </owl:Class>
    


    <!-- https://endlessforms.info/gdo/GDO_0000214 -->

    <owl:Class rdf:about="https://endlessforms.info/gdo/GDO_0000214">
        <rdfs:subClassOf rdf:resource="http://www.ontologyrepository.com/CommonCoreOntologies/DirectiveInformationContentEntity"/>
        <obo:IAO_0000115>A directive information content entity that stores data and commands in a digital format to be used by a computer to render an image.</obo:IAO_0000115>
        <rdfs:label xml:lang="en">image file</rdfs:label>
    </owl:Class>
    


    <!-- https://endlessforms.info/gdo/GDO_0000215 -->

    <owl:Class rdf:about="https://endlessforms.info/gdo/GDO_0000215">
        <rdfs:subClassOf rdf:resource="https://endlessforms.info/gdo/GDO_0000214"/>
        <obo:IAO_0000115>An image file in the Scalable Vector Graphics format.</obo:IAO_0000115>
        <rdfs:label xml:lang="en">SVG file</rdfs:label>
    </owl:Class>
    


    <!-- https://endlessforms.info/gdo/GDO_0000216 -->

    <owl:Class rdf:about="https://endlessforms.info/gdo/GDO_0000216">
        <rdfs:subClassOf rdf:resource="http://www.ontologyrepository.com/CommonCoreOntologies/DirectiveInformationContentEntity"/>
        <obo:IAO_0000115>A directive information content entity that is a component of an SVG file and provides instructions for drawing a shape.</obo:IAO_0000115>
        <rdfs:label xml:lang="en">element of an SVG file</rdfs:label>
    </owl:Class>
    


    <!-- https://endlessforms.info/gdo/GDO_0000217 -->

    <owl:Class rdf:about="https://endlessforms.info/gdo/GDO_0000217">
        <rdfs:subClassOf rdf:resource="https://endlessforms.info/gdo/GDO_0000216"/>
        <obo:IAO_0000115>An element of an SVG file that provides instructions for drawing a path.</obo:IAO_0000115>
        <rdfs:label xml:lang="en">SVG path</rdfs:label>
    </owl:Class>
    


    <!-- https://endlessforms.info/gdo/GDO_0000218 -->

    <owl:Class rdf:about="https://endlessforms.info/gdo/GDO_0000218">
        <rdfs:subClassOf rdf:resource="https://endlessforms.info/gdo/GDO_0000216"/>
        <obo:IAO_0000115>An element of an SVG file that provides instructions for drawing a rectangle.</obo:IAO_0000115>
        <rdfs:label xml:lang="en">SVG rectangle</rdfs:label>
    </owl:Class>
    


    <!-- https://endlessforms.info/gdo/GDO_0000219 -->

    <owl:Class rdf:about="https://endlessforms.info/gdo/GDO_0000219">
        <rdfs:subClassOf rdf:resource="https://endlessforms.info/gdo/GDO_0000216"/>
        <obo:IAO_0000115>An element of an SVG file that provides instructions for drawing a circle.</obo:IAO_0000115>
        <rdfs:label xml:lang="en">SVG circle</rdfs:label>
    </owl:Class>
    


    <!-- https://endlessforms.info/gdo/GDO_0000220 -->

    <owl:Class rdf:about="https://endlessforms.info/gdo/GDO_0000220">
        <rdfs:subClassOf rdf:resource="https://endlessforms.info/gdo/GDO_0000216"/>
        <obo:IAO_0000115>An element of an SVG file that provides instructions for drawing an ellipse.</obo:IAO_0000115>
        <rdfs:label xml:lang="en">SVG ellipse</rdfs:label>
    </owl:Class>
    


    <!-- https://endlessforms.info/gdo/GDO_0000221 -->

    <owl:Class rdf:about="https://endlessforms.info/gdo/GDO_0000221">
        <rdfs:subClassOf rdf:resource="https://endlessforms.info/gdo/GDO_0000216"/>
        <obo:IAO_0000115>An element of an SVG file that provides instructions for drawing a line.</obo:IAO_0000115>
        <rdfs:label xml:lang="en">SVG line</rdfs:label>
    </owl:Class>
    


    <!-- https://endlessforms.info/gdo/GDO_0000222 -->

    <owl:Class rdf:about="https://endlessforms.info/gdo/GDO_0000222">
        <rdfs:subClassOf rdf:resource="https://endlessforms.info/gdo/GDO_0000216"/>
        <obo:IAO_0000115>An element of an SVG file that provides instructions for drawing a polyline.</obo:IAO_0000115>
        <rdfs:label xml:lang="en">SVG polyline</rdfs:label>
    </owl:Class>
    


    <!-- https://endlessforms.info/gdo/GDO_0000223 -->

    <owl:Class rdf:about="https://endlessforms.info/gdo/GDO_0000223">
        <rdfs:subClassOf rdf:resource="https://endlessforms.info/gdo/GDO_0000216"/>
        <obo:IAO_0000115>An element of an SVG file that provides instructions for drawing a polygon.</obo:IAO_0000115>
        <rdfs:label xml:lang="en">SVG polygon</rdfs:label>
    </owl:Class>
    


    <!-- https://endlessforms.info/gdo/GDO_0000224 -->

    <owl:Class rdf:about="https://endlessforms.info/gdo/GDO_0000224">
        <rdfs:subClassOf rdf:resource="https://endlessforms.info/gdo/GDO_0000214"/>
        <obo:IAO_0000115>An image file in the Joint Photographic Experts Group format. This is a type of raster file.</obo:IAO_0000115>
        <obo:IAO_0000118>JPEG file</obo:IAO_0000118>
        <rdfs:label xml:lang="en">JPG file</rdfs:label>
    </owl:Class>
    


    <!-- https://endlessforms.info/gdo/GDO_0000225 -->

    <owl:Class rdf:about="https://endlessforms.info/gdo/GDO_0000225">
        <rdfs:subClassOf rdf:resource="https://endlessforms.info/gdo/GDO_0000214"/>
        <obo:IAO_0000115>An image file in the Portable Network Graphic format. This is a type of raster file.</obo:IAO_0000115>
        <rdfs:label xml:lang="en">PNG file</rdfs:label>
    </owl:Class>
    


    <!-- https://endlessforms.info/gdo/GDO_0000226 -->

    <owl:Class rdf:about="https://endlessforms.info/gdo/GDO_0000226">
        <rdfs:subClassOf rdf:resource="https://endlessforms.info/gdo/GDO_0000214"/>
        <obo:IAO_0000115>An image file in the Graphics Interchange Format. This is a type of raster file.</obo:IAO_0000115>
        <rdfs:label xml:lang="en">GIF file</rdfs:label>
    </owl:Class>
    


    <!-- https://endlessforms.info/gdo/GDO_0000235 -->

    <owl:Class rdf:about="https://endlessforms.info/gdo/GDO_0000235">
        <rdfs:subClassOf rdf:resource="https://endlessforms.info/gdo/GDO_0000064"/>
        <obo:IAO_0000115>A line mark role for which the mark designates a line deemed to be particularly important for the communication purpose of the graphic.</obo:IAO_0000115>
        <rdfs:label xml:lang="en">line of interest</rdfs:label>
    </owl:Class>
    


    <!-- https://endlessforms.info/gdo/GDO_0000237 -->

    <owl:Class rdf:about="https://endlessforms.info/gdo/GDO_0000237">
        <rdfs:subClassOf rdf:resource="http://www.ontologyrepository.com/CommonCoreOntologies/InformationBearingEntity"/>
        <obo:IAO_0000115>An information bearing entity that is a pictorial model of information, such that the spatial arrangement of graphical marks (or other units, such as pixels) corresponds to the form of referent. May also represent other qualitites of the referent that an be perceived visually, such as color, value, and texture.</obo:IAO_0000115>
        <obo:IAO_0000116>This class includes both graphics and photos.</obo:IAO_0000116>
        <rdfs:label xml:lang="en">pictorial information bearing entity</rdfs:label>
    </owl:Class>
    


    <!-- https://endlessforms.info/gdo/GDO_0000250 -->

    <owl:Class rdf:about="https://endlessforms.info/gdo/GDO_0000250">
        <rdfs:subClassOf rdf:resource="https://endlessforms.info/gdo/GDO_0000072"/>
        <obo:IAO_0000115>A ridge line characterized by a sudden change in surface normal when crossing the ridge line.</obo:IAO_0000115>
        <rdfs:label xml:lang="en">sharp ridge line</rdfs:label>
    </owl:Class>
    


    <!-- https://endlessforms.info/gdo/GDO_0000251 -->

    <owl:Class rdf:about="https://endlessforms.info/gdo/GDO_0000251">
        <rdfs:subClassOf rdf:resource="https://endlessforms.info/gdo/GDO_0000071"/>
        <obo:IAO_0000115>A valley line characterized by a sudden change in surface normal when crossing the valley line.</obo:IAO_0000115>
        <rdfs:label xml:lang="en">sharp valley line</rdfs:label>
    </owl:Class>
    


    <!-- 
    ///////////////////////////////////////////////////////////////////////////////////////
    //
    // Individuals
    //
    ///////////////////////////////////////////////////////////////////////////////////////
     -->

    


    <!-- https://endlessforms.info/gdo/GDO_0000017 -->

    <owl:NamedIndividual rdf:about="https://endlessforms.info/gdo/GDO_0000017">
        <rdf:type rdf:resource="https://endlessforms.info/gdo/GDO_0000026"/>
        <obo:IAO_0000115>A style of representation of parts in which part or all of the surface of a referent is depicted as transparent so that its internal parts are revealed.</obo:IAO_0000115>
        <rdfs:label xml:lang="en">style of transparency of exterior</rdfs:label>
    </owl:NamedIndividual>
    


    <!-- https://endlessforms.info/gdo/GDO_0000020 -->

    <owl:NamedIndividual rdf:about="https://endlessforms.info/gdo/GDO_0000020">
        <rdf:type rdf:resource="https://endlessforms.info/gdo/GDO_0000018"/>
        <obo:IAO_0000115>An orthographic view depicting the back of a referent.</obo:IAO_0000115>
        <rdfs:label xml:lang="en">orthographic back view</rdfs:label>
    </owl:NamedIndividual>
    


    <!-- https://endlessforms.info/gdo/GDO_0000021 -->

    <owl:NamedIndividual rdf:about="https://endlessforms.info/gdo/GDO_0000021">
        <rdf:type rdf:resource="https://endlessforms.info/gdo/GDO_0000018"/>
        <obo:IAO_0000115>An orthographic view depicting the front of a referent.</obo:IAO_0000115>
        <rdfs:label xml:lang="en">orthographic front view</rdfs:label>
    </owl:NamedIndividual>
    


    <!-- https://endlessforms.info/gdo/GDO_0000022 -->

    <owl:NamedIndividual rdf:about="https://endlessforms.info/gdo/GDO_0000022">
        <rdf:type rdf:resource="https://endlessforms.info/gdo/GDO_0000018"/>
        <obo:IAO_0000115>An orthographic view depicting the left side of a referent.</obo:IAO_0000115>
        <rdfs:label xml:lang="en">orthographic left side view</rdfs:label>
    </owl:NamedIndividual>
    


    <!-- https://endlessforms.info/gdo/GDO_0000023 -->

    <owl:NamedIndividual rdf:about="https://endlessforms.info/gdo/GDO_0000023">
        <rdf:type rdf:resource="https://endlessforms.info/gdo/GDO_0000018"/>
        <obo:IAO_0000115>An orthographic view depicting the right side of a referent.</obo:IAO_0000115>
        <rdfs:label xml:lang="en">orthographic right side view</rdfs:label>
    </owl:NamedIndividual>
    


    <!-- https://endlessforms.info/gdo/GDO_0000024 -->

    <owl:NamedIndividual rdf:about="https://endlessforms.info/gdo/GDO_0000024">
        <rdf:type rdf:resource="https://endlessforms.info/gdo/GDO_0000018"/>
        <obo:IAO_0000115>An orthographic view depicting the bottom of a referent.</obo:IAO_0000115>
        <rdfs:label xml:lang="en">orthographic bottom view</rdfs:label>
    </owl:NamedIndividual>
    


    <!-- https://endlessforms.info/gdo/GDO_0000025 -->

    <owl:NamedIndividual rdf:about="https://endlessforms.info/gdo/GDO_0000025">
        <rdf:type rdf:resource="https://endlessforms.info/gdo/GDO_0000018"/>
        <obo:IAO_0000115>An orthographic view depicting the top of a referent.</obo:IAO_0000115>
        <rdfs:label xml:lang="en">orthographic top view</rdfs:label>
    </owl:NamedIndividual>
    


    <!-- https://endlessforms.info/gdo/GDO_0000027 -->

    <owl:NamedIndividual rdf:about="https://endlessforms.info/gdo/GDO_0000027">
        <rdf:type rdf:resource="https://endlessforms.info/gdo/GDO_0000026"/>
        <obo:IAO_0000115>A style of representation of parts in which the outline of a referent is drawn to give positional context to its internal parts that are the subject matter of the representation.</obo:IAO_0000115>
        <rdfs:label xml:lang="en">style of reference contour</rdfs:label>
    </owl:NamedIndividual>
    


    <!-- https://endlessforms.info/gdo/GDO_0000028 -->

    <owl:NamedIndividual rdf:about="https://endlessforms.info/gdo/GDO_0000028">
        <rdf:type rdf:resource="https://endlessforms.info/gdo/GDO_0000026"/>
        <obo:IAO_0000115>A style of representation of parts in which a section, slice, or block is drawn as if excised from a referent so that its internal parts are revealed.</obo:IAO_0000115>
        <rdfs:label xml:lang="en">style of extracted section</rdfs:label>
    </owl:NamedIndividual>
    


    <!-- https://endlessforms.info/gdo/GDO_0000029 -->

    <owl:NamedIndividual rdf:about="https://endlessforms.info/gdo/GDO_0000029">
        <rdf:type rdf:resource="https://endlessforms.info/gdo/GDO_0000026"/>
        <obo:IAO_0000115>A style of representation of parts in which a portion of the surface of a referent is depicted as absent so that its internal parts are revealed.</obo:IAO_0000115>
        <rdfs:label xml:lang="en">style of cut-away of exterior</rdfs:label>
    </owl:NamedIndividual>
    


    <!-- https://endlessforms.info/gdo/GDO_0000030 -->

    <owl:NamedIndividual rdf:about="https://endlessforms.info/gdo/GDO_0000030">
        <rdf:type rdf:resource="https://endlessforms.info/gdo/GDO_0000026"/>
        <obo:IAO_0000115>A style of representation of parts in which parts of a referent are drawn displaced from their natural locations so that the viewer can differentiate individual parts.</obo:IAO_0000115>
        <rdfs:label xml:lang="en">style of exploded parts</rdfs:label>
    </owl:NamedIndividual>
    


    <!-- https://endlessforms.info/gdo/GDO_0000031 -->

    <owl:NamedIndividual rdf:about="https://endlessforms.info/gdo/GDO_0000031">
        <rdf:type rdf:resource="https://endlessforms.info/gdo/GDO_0000026"/>
        <obo:IAO_0000115>A style of representation of parts in which multiple sections of a referent are displayed, in their natural order, so that its internal parts are revealed.</obo:IAO_0000115>
        <rdfs:label xml:lang="en">style of serial sections</rdfs:label>
    </owl:NamedIndividual>
    


    <!-- https://endlessforms.info/gdo/GDO_0000035 -->

    <owl:NamedIndividual rdf:about="https://endlessforms.info/gdo/GDO_0000035">
        <rdf:type rdf:resource="https://endlessforms.info/gdo/GDO_0000034"/>
        <obo:IAO_0000115>A graphic style in which the graphical marks have a natural a resemblance to the physical form of the referent, such that the marks directly correspond to the contours and other spatial characteristics of the referent.</obo:IAO_0000115>
        <rdfs:label xml:lang="en">naturalistic style</rdfs:label>
    </owl:NamedIndividual>
    


    <!-- https://endlessforms.info/gdo/GDO_0000036 -->

    <owl:NamedIndividual rdf:about="https://endlessforms.info/gdo/GDO_0000036">
        <rdf:type rdf:resource="https://endlessforms.info/gdo/GDO_0000034"/>
        <obo:IAO_0000115>A graphic style in which the graphical marks have an indirect resemblance to the physical form of the referent, such that the marks correspond only partially to the contours and other spatial characteristics of the referent. Graphics that have a diagrammatic style communicate some information about the physical form of the referent or its parts, but this information is simplified and abstracted.</obo:IAO_0000115>
        <rdfs:label xml:lang="en">diagrammatic style</rdfs:label>
    </owl:NamedIndividual>
    


    <!-- https://endlessforms.info/gdo/GDO_0000039 -->

    <owl:NamedIndividual rdf:about="https://endlessforms.info/gdo/GDO_0000039">
        <rdf:type rdf:resource="https://endlessforms.info/gdo/GDO_0000038"/>
        <obo:IAO_0000115>A type of parallel projection for which the lines of sight are not perpendicular to the plane of projection (the imaginary flat plane onto which a representation of the referent is projected).</obo:IAO_0000115>
        <rdfs:label xml:lang="en">oblique projection</rdfs:label>
    </owl:NamedIndividual>
    


    <!-- https://endlessforms.info/gdo/GDO_0000040 -->

    <owl:NamedIndividual rdf:about="https://endlessforms.info/gdo/GDO_0000040">
        <rdf:type rdf:resource="https://endlessforms.info/gdo/GDO_0000038"/>
        <obo:IAO_0000115>A type of parallel projection for which the lines of sight are perpendicular to the plane of projection (the imaginary flat plane onto which a representation of the referent is projected).</obo:IAO_0000115>
        <rdfs:label xml:lang="en">orthographic projection</rdfs:label>
    </owl:NamedIndividual>
    


    <!-- https://endlessforms.info/gdo/GDO_0000042 -->

    <owl:NamedIndividual rdf:about="https://endlessforms.info/gdo/GDO_0000042">
        <rdf:type rdf:resource="https://endlessforms.info/gdo/GDO_0000041"/>
        <obo:IAO_0000115>A perspective projection for which all three principal axes intersect with the plane of projection. Projection lines parallel to the three axes converge at three vanishing points. No axes are parallel to the plane of projection.</obo:IAO_0000115>
        <rdfs:label xml:lang="en">3-point perspective</rdfs:label>
    </owl:NamedIndividual>
    


    <!-- https://endlessforms.info/gdo/GDO_0000043 -->

    <owl:NamedIndividual rdf:about="https://endlessforms.info/gdo/GDO_0000043">
        <rdf:type rdf:resource="https://endlessforms.info/gdo/GDO_0000041"/>
        <obo:IAO_0000115>A perspective projection for which two of the principal axes intersect with the plane of projection. Projection lines parallel to these two axes converge at two vanishing points. The third axis is parallel to the plane of projection.</obo:IAO_0000115>
        <rdfs:label xml:lang="en">2-point perspective</rdfs:label>
    </owl:NamedIndividual>
    


    <!-- https://endlessforms.info/gdo/GDO_0000044 -->

    <owl:NamedIndividual rdf:about="https://endlessforms.info/gdo/GDO_0000044">
        <rdf:type rdf:resource="https://endlessforms.info/gdo/GDO_0000041"/>
        <obo:IAO_0000115>A perspective projection for which the principal axes receding into the distance intersects with the plane of projection. Projection lines parallel to this receding axis converge at a point called the vanishing point. The horizontal and vertical axes are parallel to the plane of projection.</obo:IAO_0000115>
        <rdfs:label xml:lang="en">1-point perspective</rdfs:label>
    </owl:NamedIndividual>
</rdf:RDF>



<!-- Generated by the OWL API (version 4.5.9.2019-02-01T07:24:44Z) https://github.com/owlcs/owlapi -->

